## subset
### number of subset
- 2 ** n

### powerset by backtracking
recursion
```python
def f(i, n):
    if i == n:
        print(B)
        return
    else:
        B[i] = A[i]
        f(i + 1, n)


N = 3
A = [n for n in range(1, N + 1)]
B = [0] * N
f(0, N)
```

subset recursion
```python
def f(i, n):
    if i == n:
        print(bit, end=" ")
        s = 0
        for j in range(n):
            if bit[j]:
                s += A[j]
                print(A[j], end=" ")
        print(f" : {s}")
        return
    else:
        bit[i] = 1
        f(i + 1, n)
        bit[i] = 0
        f(i + 1, n)
        return


A = [1, 2, 3]
bit = [0] * 3
f(0, 3)
```

subset sum recursion
```python
def f(i, n, s):  # s : subset sum to i-1
    if i == n:
        print(bit, end=" ")
        print(f" : {s}")
        return
    else:
        bit[i] = 1
        f(i + 1, n, s + A[i])
        bit[i] = 0
        f(i + 1, n, s)
        return


A = [1, 2, 3]
bit = [0] * 3
f(0, 3, 0)
```

### practice
```python
def f(i, n, s, t):  # s : subset sum to i-1, t : target sum
    global cnt
    cnt += 1
    if s == t:
        print(bit)
        return
    elif i == N:
        return
    elif s > t:
        return
    else:
        bit[i] = 1
        f(i + 1, n, s + A[i], t)
        bit[i] = 0
        f(i + 1, n, s, t)
        return


N = 10
A = [i for i in range(1, N + 1)]
bit = [0] * N
cnt = 0
f(0, N, 0, 1)
print(cnt)
```

## permutation
### permutation algorithm
```python
def f(i, n):
    if i == n:
        print(A)
    else:
        for j in range(i, n):  # from itself to the right end
            A[i], A[j] = A[j], A[i]
            f(i + 1, n)
            A[i], A[j] = A[j], A[i]


A = [0, 1, 2]
f(0, 3)
```

## divide and conquer algorithm
### strategy
- divide
- conquer
- combine

### examples
- exponentitation
- O(log2n)

### algorithm
```python
def f1(b, e):
    global cnt1
    if b == 0:
        cnt1 += 1
    r = 1
    for i in range(e):
        cnt1 += 1
        r *= b
    return r


def f2(b, e):
    global cnt2
    if b == 0 or e == 0:
        return 1
    if e % 2:
        r = f2(b, (e - 1) // 2)
        cnt2 += 1
        return r * r * b
    else:
        r = f2(b, e // 2)
        cnt2 += 1
        return r * r


cnt1 = 0
cnt2 = 0
print(f1(2, 10), cnt1)
print(f2(2, 10), cnt2)
```